vc/heap/pop/ret_path1_verif.v
@@ -13,13 +13,10 @@ Theorem proof: functional_correctness_statement.
 Proof.
   cbv delta [functional_correctness_statement].
   intros; Intros; subst.
-  forward. forward. forward. 
+  forward. forward. forward.
   sep_apply list_length; [lia|].
   Intros.
-  forward.
-  (* forward. forward.
-  forward. forward.
-  forward_call (size0-1, 1, a0, Maxsize, Hl, a0, (Vint (IntRepr 1)), (Vint (Int.sub (IntRepr size0) (IntRepr 1)))). *)
+  forward. forward. forward. forward. forward.
 Admitted.
 
 End SH_Proof.
