vc/heap/push/path0_verif.v
@@ -13,10 +13,8 @@ Theorem proof: functional_correctness_statement.
 Proof.
   cbv delta [functional_correctness_statement].
   intros; Intros; subst.
-  forward.
-  (* unfold POSTCONDITION.
-  unfold abbreviate. *)
-  (* forward.  *)
+  forward. forward. forward. forward. forward.
+  forward_call ((size0+1), (size0+1), a', Maxsize, Hl ++ [val0], a', (Vint (IntRepr (size0+1)))).
   
 Admitted.
 
